Remove `MonadMorphism`

MPL/WPMonad.lean
@@ -4,12 +4,12 @@ Released under Apache 2.0 license as described in the file LICENSE.
 Authors: Sebastian Graf
 -/
 import MPL.WP
-import MPL.MonadMorphism
 
 /-!
 # Monad morphisms and weakest precondition interpretations
 
-A `WP m ps` is a `WPMonad m ps` if the interpretation `WP.wp` is also a `MonadMorphism`.
+A `WP m ps` is a `WPMonad m ps` if the interpretation `WP.wp` is also a monad morphism, that is,
+it preserves `pure` and `bind`.
 -/
 
 namespace MPL
@@ -19,80 +19,86 @@ universe u
 variable {m : Type → Type u} {ps : PostShape}
 
 /--
-  A `WP` that is also a `MonadMorphism`. (They all are.)
+  A `WP` that is also a monad morphism, preserving `pure` and `bind`. (They all are.)
 -/
 class WPMonad (m : Type → Type u) (ps : outParam PostShape) [Monad m]
-  extends LawfulMonad m, WP m ps, MonadMorphism m (PredTrans ps) wp where
+  extends LawfulMonad m, WP m ps where
+  wp_pure : ∀ {α} (a : α), wp (pure a) = pure a
+  wp_bind : ∀ {α β} (x : m α) (f : α → m β), wp (do let a ← x; f a) = do let a ← wp x; wp (f a)
 
-theorem WP.pure_apply [Monad m] [WPMonad m ps] (a : α) (Q : PostCond α ps) :
-  wp⟦pure (f:=m) a⟧ Q = let x := a; Q.1 x := by
-    simp only [pure_pure, PredTrans.pure_apply]
+attribute [simp] WPMonad.wp_pure WPMonad.wp_bind
 
-theorem WP.bind_apply [Monad m] [WPMonad m ps] (x : m α) (f : α → m β) (Q : PostCond β ps) :
+@[simp]
+theorem WPMonad.wp_map [Monad m] [WPMonad m ps] (f : α → β) (x : m α) :
+  wp (f <$> x) = f <$> wp x := by
+    simp [← bind_pure_comp, wp_bind, wp_pure]
+
+@[simp]
+theorem WPMonad.wp_seq [Monad m] [WPMonad m ps] (f : m (α → β)) (x : m α) :
+  wp (f <*> x) = wp f <*> wp x := by
+    simp [← bind_map, wp_bind, wp_map]
+
+@[simp]
+theorem WPMonad.wp_dite {c : Prop} [Decidable c] {t : c → m α} {e : ¬c → m α} [Monad m] [WPMonad m ps] :
+  wp (dite c t e) = if h : c then wp (t h) else wp (e h) := by
+    split <;> simp
+
+@[simp]
+theorem WPMonad.wp_ite {c : Prop} [Decidable c] {t : m α} {e : m α} [Monad m] [WPMonad m ps] :
+  wp (ite c t e) = if c then wp t else wp e := by
+  split <;> simp
+
+theorem WPMonad.pure_apply [Monad m] [WPMonad m ps] (a : α) (Q : PostCond α ps) :
+  wp⟦pure (f:=m) a⟧ Q = Q.1 a := by
+    simp only [wp_pure, PredTrans.pure_apply]
+
+theorem WPMonad.bind_apply [Monad m] [WPMonad m ps] (x : m α) (f : α → m β) (Q : PostCond β ps) :
   wp⟦x >>= f⟧ Q = wp⟦x⟧ (fun a => wp⟦f a⟧ Q, Q.2) := by
-    simp only [bind_bind, PredTrans.bind_apply]
+    simp only [wp_bind, PredTrans.bind_apply]
 
-theorem WP.map_apply [Monad m] [WPMonad m ps] (f : α → β) (x : m α) (Q : PostCond β ps) :
+theorem WPMonad.map_apply [Monad m] [WPMonad m ps] (f : α → β) (x : m α) (Q : PostCond β ps) :
   wp⟦f <$> x⟧ Q = wp⟦x⟧ (fun a => Q.1 (f a), Q.2) := by
-    simp only [map_map, PredTrans.map_apply]
+    simp only [wp_map, PredTrans.map_apply]
 
-theorem WP.seq_apply [Monad m] [WPMonad m ps] (f : m (α → β)) (x : m α) (Q : PostCond β ps) :
+theorem WPMonad.seq_apply [Monad m] [WPMonad m ps] (f : m (α → β)) (x : m α) (Q : PostCond β ps) :
   wp⟦f <*> x⟧ Q = wp⟦f⟧ (fun f => wp⟦x⟧ (fun a => Q.1 (f a), Q.2), Q.2) := by
-    simp only [seq_seq, PredTrans.seq_apply]
+    simp only [wp_seq, PredTrans.seq_apply]
 
-theorem WP.morph_pure_apply [Monad m] [Monad n] [LawfulMonad m] [MonadMorphism m n morph] [WPMonad n ps]
-  (a : α) (Q : PostCond α ps) :
-  wp⟦morph (pure a) : n α⟧ Q = wp⟦pure a : n α⟧ Q := by
-    simp only [pure_pure]
+theorem WPMonad.dite_apply {ps} {Q : PostCond α ps} (c : Prop) [Decidable c] [Monad m] [WPMonad m ps] (t : c → m α) (e : ¬ c → m α) :
+  wp⟦if h : c then t h else e h⟧ Q = if h : c then wp⟦t h⟧ Q else wp⟦e h⟧ Q := by split <;> rfl
 
-theorem WP.morph_bind_apply [Monad m] [Monad n] [LawfulMonad m] [MonadMorphism m n morph] [WPMonad n ps]
-  (x : m α) (f : α → m β) (Q : PostCond β ps) :
-  wp⟦morph (x >>= f) : n β⟧ Q = wp⟦morph x >>= fun a => morph (f a) : n β⟧ Q := by
-    simp only [bind_bind]
+theorem WPMonad.ite_apply {ps} {Q : PostCond α ps} (c : Prop) [Decidable c] [Monad m] [WPMonad m ps] (t : m α) (e : m α) :
+  wp⟦if c then t else e⟧ Q = if c then wp⟦t⟧ Q else wp⟦e⟧ Q := by split <;> rfl
 
-theorem WP.morph_map_apply [Monad m] [Monad n] [LawfulMonad m] [MonadMorphism m n morph] [WPMonad n ps]
-  (f : α → β) (x : m α) (Q : PostCond β ps) :
-  wp⟦morph (f <$> x) : n β⟧ Q = wp⟦f <$> morph x : n β⟧ Q := by
-    simp only [map_map]
-
-theorem WP.morph_seq_apply [Monad m] [Monad n] [LawfulMonad m] [MonadMorphism m n morph] [WPMonad n ps]
-  (f : m (α → β)) (x : m α) (Q : PostCond β ps) :
-  wp⟦morph (f <*> x) : n β⟧ Q = wp⟦morph f <*> morph x : n β⟧ Q := by
-    simp only [seq_seq]
-
-theorem WP.morph_dite_apply {ps} {Q : PostCond α ps} (c : Prop) [Decidable c] [Monad m] [Monad n] [MonadMorphism m n morph] [WP n ps] (t : c → m α) (e : ¬ c → m α) :
-  wp⟦morph (if h : c then t h else e h)⟧ Q = if h : c then wp⟦morph (t h)⟧ Q else wp⟦morph (e h)⟧ Q := by split <;> rfl
-
-theorem WP.morph_ite_apply {ps} {Q : PostCond α ps} (c : Prop) [Decidable c] [Monad m] [Monad n] [MonadMorphism m n morph] [WP n ps] (t : m α) (e : m α) :
-  wp⟦morph (if c then t else e)⟧ Q = if c then wp⟦morph t⟧ Q else wp⟦morph e⟧ Q := by split <;> rfl
+open WPMonad
 
 instance Idd.instWPMonad : WPMonad Idd .pure where
-  pure_pure a := by ext; simp only [wp, Idd.run_pure, instMonadPredTrans]
-  bind_bind x f := by ext; simp only [wp, PredTrans.pure, Bind.bind, Idd.bind, PredTrans.bind]
+  wp_pure a := by ext; simp only [wp, Idd.run_pure, instMonadPredTrans]
+  wp_bind x f := by ext; simp only [wp, PredTrans.pure, Bind.bind, Idd.bind, PredTrans.bind]
 
 instance Id.instWPMonad : WPMonad Id .pure where
-  pure_pure a := by simp only [wp, PredTrans.pure, Pure.pure, Id.run]
-  bind_bind x f := by simp only [wp, PredTrans.pure, Bind.bind, Id.run, PredTrans.bind]
+  wp_pure a := by simp only [wp, PredTrans.pure, Pure.pure, Id.run]
+  wp_bind x f := by simp only [wp, PredTrans.pure, Bind.bind, Id.run, PredTrans.bind]
 
 instance StateT.instWPMonad [Monad m] [WPMonad m ps] : WPMonad (StateT σ m) (.arg σ ps) where
-  pure_pure a := by ext; simp only [wp, pure, StateT.pure, pure_pure, PredTrans.pure,
+  wp_pure a := by ext; simp only [wp, pure, StateT.pure, WPMonad.wp_pure, PredTrans.pure,
     PredTrans.pushArg_apply]
-  bind_bind x f := by ext; simp only [wp, bind, StateT.bind, bind_bind, PredTrans.bind,
+  wp_bind x f := by ext; simp only [wp, bind, StateT.bind, WPMonad.wp_bind, PredTrans.bind,
     PredTrans.pushArg_apply]
 
 instance ReaderT.instWPMonad [Monad m] [WPMonad m ps] : WPMonad (ReaderT ρ m) (.arg ρ ps) where
-  pure_pure a := by ext; simp only [wp, pure, ReaderT.pure, pure_pure, PredTrans.pure,
+  wp_pure a := by ext; simp only [wp, pure, ReaderT.pure, WPMonad.wp_pure, PredTrans.pure,
     PredTrans.pushArg_apply, PredTrans.map_apply]
-  bind_bind x f := by ext; simp only [wp, bind, ReaderT.bind, bind_bind, PredTrans.bind,
+  wp_bind x f := by ext; simp only [wp, bind, ReaderT.bind, WPMonad.wp_bind, PredTrans.bind,
     PredTrans.pushArg_apply, PredTrans.map_apply]
 
 instance ExceptT.instWPMonad [Monad m] [WPMonad m ps] : WPMonad (ExceptT ε m) (.except ε ps) where
-  pure_pure a := by ext; simp only [wp, pure, ExceptT.pure, ExceptT.mk, pure_pure, PredTrans.pure,
-    PredTrans.pushExcept_apply]
-  bind_bind x f := by
+  wp_pure a := by ext; simp only [wp, pure, ExceptT.pure, ExceptT.mk, WPMonad.wp_pure,
+    PredTrans.pure, PredTrans.pushExcept_apply]
+  wp_bind x f := by
     ext Q
-    simp only [wp, bind, ExceptT.bind, ExceptT.mk, bind_bind, PredTrans.bind, ExceptT.bindCont,
-      PredTrans.pushExcept_apply]
+    simp only [wp, bind, ExceptT.bind, ExceptT.mk, WPMonad.wp_bind, PredTrans.bind,
+      ExceptT.bindCont, PredTrans.pushExcept_apply]
     congr
     ext b
     cases b
@@ -100,16 +106,16 @@ instance ExceptT.instWPMonad [Monad m] [WPMonad m ps] : WPMonad (ExceptT ε m) (
     case ok a => rfl
 
 instance EStateM.instWPMonad : WPMonad (EStateM ε σ) (.except ε (.arg σ .pure)) where
-  pure_pure a := by simp only [wp, pure, EStateM.pure, PredTrans.pure]
-  bind_bind x f := by
+  wp_pure a := by simp only [wp, pure, EStateM.pure, PredTrans.pure]
+  wp_bind x f := by
     ext Q : 2
     simp [wp, bind, EStateM.bind, eq_iff_iff, PredTrans.bind]
     ext s : 1
     cases (x s) <;> simp
 
 instance Except.instWPMonad : WPMonad (Except ε) (.except ε .pure) where
-  pure_pure a := rfl
-  bind_bind x f := by cases x <;> rfl
+  wp_pure a := rfl
+  wp_bind x f := by cases x <;> rfl
 
 instance State.instWPMonad : WPMonad (StateM σ) (.arg σ .pure) :=
   inferInstanceAs (WPMonad (StateT σ Id) (.arg σ .pure))
