MPL/WPMonadLift.lean
@@ -17,12 +17,14 @@ namespace MPL
 universe u
 variable {m : Type → Type u} {ps : PostShape}
 
+open WPMonad
+
 -- The next 3 instances are important to interpret away monadLift.
 -- Note that we manage to map from `wp⟦·⟧ Q` to `wp⟦·⟧ (... Q ...)`
 -- (modulo `fun s =>`) so that the next wp_simp rule immediately applies
 theorem StateT.monadLift_apply [Monad m] [WPMonad m ps] (x : m α) (Q : PostCond α (.arg σ ps)) :
   wp⟦MonadLift.monadLift x : StateT σ m α⟧ Q = fun s => wp⟦x⟧ (fun a => Q.1 a s, Q.2) := by
-    simp only [wp, MonadLift.monadLift, StateT.lift, bind_pure_comp, map_map,
+    simp only [wp, MonadLift.monadLift, StateT.lift, bind_pure_comp, wp_map,
       PredTrans.pushArg_apply, PredTrans.map_apply]
 
 theorem ReaderT.monadLift_apply [Monad m] [WPMonad m ps] (x : m α) (Q : PostCond α (.arg ρ ps)) :
@@ -31,7 +33,7 @@ theorem ReaderT.monadLift_apply [Monad m] [WPMonad m ps] (x : m α) (Q : PostCon
 
 theorem ExceptT.monadLift_apply [Monad m] [WPMonad m ps] (x : m α) (Q : PostCond α (.except ε ps)) :
   wp⟦MonadLift.monadLift x : ExceptT ε m α⟧ Q = wp⟦x⟧ (fun a => Q.1 a, Q.2.2) := by
-    simp only [wp, MonadLift.monadLift, ExceptT.lift, ExceptT.mk, map_map,
+    simp only [wp, MonadLift.monadLift, ExceptT.lift, ExceptT.mk, wp_map,
       PredTrans.pushExcept_apply, PredTrans.map_apply]
 
 theorem MonadLiftT.monadLift_trans_apply [WP o ps] [MonadLift n o] [MonadLiftT m n] :
@@ -42,27 +44,11 @@ theorem MonadLiftT.monadLift_refl_apply [WP m ps] :
   wp⟦MonadLiftT.monadLift x : m α⟧ Q = wp⟦x : m α⟧ Q := by
     simp only [MonadLiftT.monadLift]
 
--- The following instance is useful when we want to derive `modify f = monadLift (modify f)` and `modify f`
--- is defined in terms of multiple primitive definitions in `m` (`get`, `set`, ...), rather than just one call to `modifyGet`.
--- Example: `MonadStateOf.mkFreshNat_apply` in Tests/Toy.lean
--- The alternative would be to have one lemma for concrete transformer stack at which `mkFreshNat_apply` is used that simply unfolds the definition.
-instance StateT.instLiftMonadMorphism [Monad m] [LawfulMonad m] : MonadMorphism m (StateT σ m) MonadLift.monadLift where
-  pure_pure x := by ext; simp [liftM, MonadLift.monadLift, StateT.lift]
-  bind_bind x f := by ext; simp [liftM, MonadLift.monadLift, StateT.lift]
-
-instance ReaderT.instLiftMonadMorphism [Monad m] [LawfulMonad m] : MonadMorphism m (ReaderT ρ m) MonadLift.monadLift where
-  pure_pure x := by ext; simp [liftM, MonadLift.monadLift, ReaderT.run, pure, ReaderT.pure]
-  bind_bind x f := by ext; simp [liftM, MonadLift.monadLift, ReaderT.run, bind, ReaderT.bind]
-
-instance ExceptT.instLiftMonadMorphism [Monad m] [LawfulMonad m] : MonadMorphism m (ExceptT ε m) MonadLift.monadLift where
-  pure_pure x := by ext; simp only [MonadLift.monadLift, ExceptT.lift, map_pure, ExceptT.run_pure]; rfl
-  bind_bind x f := by ext; simp [liftM, MonadLift.monadLift, ExceptT.lift, ExceptT.mk, bind, ExceptT.bind, ExceptT.bindCont]
-
 -- Now rewrites for the standard lib:
 
 theorem ReaderT.read_apply [Monad m] [WPMonad m psm] :
   wp⟦MonadReaderOf.read : ReaderT ρ m ρ⟧ Q = fun r => Q.1 r r  := by
-    ext; simp only [wp, MonadReaderOf.read, ReaderT.read, pure_pure, pure, PredTrans.pure,
+    ext; simp [wp, MonadReaderOf.read, ReaderT.read, WPMonad.wp_pure, pure, PredTrans.pure,
       PredTrans.pushArg_apply, PredTrans.map_apply]
 
 theorem MonadReaderOf.read_apply [MonadReaderOf ρ m] [MonadLift m n] [WP n _] :
@@ -78,12 +64,12 @@ theorem MonadReader.read_apply [MonadReaderOf ρ m] [WP m sh] :
 
 theorem StateT.get_apply [Monad m] [WPMonad m psm] :
   wp⟦MonadStateOf.get : StateT σ m σ⟧ Q = fun s => Q.1 s s := by
-    ext; simp only [wp, MonadStateOf.get, StateT.get, pure_pure, pure, PredTrans.pure,
+    ext; simp [wp, MonadStateOf.get, StateT.get, WPMonad.wp_pure, pure, PredTrans.pure,
       PredTrans.pushArg_apply]
 
 theorem EStateM.get_apply :
     wp⟦MonadStateOf.get : EStateM ε σ σ⟧ Q = fun s => Q.1 s s := by
-  ext; simp only [wp, MonadStateOf.get, EStateM.get]
+  ext; simp [wp, MonadStateOf.get, EStateM.get]
 
 theorem MonadStateOf.get_apply [MonadStateOf σ m] [MonadLift m n] [WP n _] :
   wp⟦MonadStateOf.get : n σ⟧ Q = wp⟦MonadLift.monadLift (MonadStateOf.get : m σ) : n σ⟧ Q := rfl
@@ -94,14 +80,14 @@ theorem MonadStateOf.getThe_apply [WP m sh] [MonadStateOf σ m] :
 theorem MonadState.get_apply [WP m sh] [MonadStateOf σ m] :
   wp⟦MonadState.get : m σ⟧ Q = wp⟦MonadStateOf.get : m σ⟧ Q := rfl
 
-theorem StateT.set_apply [WP m sh] [Monad m] [MonadMorphism m _ wp] (x : σ) :
+theorem StateT.set_apply [Monad m] [WPMonad m sh] (x : σ) :
   wp⟦MonadStateOf.set x : StateT σ m PUnit⟧ Q = fun _ => Q.1 ⟨⟩ x := by
-    ext; simp only [wp, MonadState.set, set, StateT.set, pure_pure, pure, PredTrans.pure,
+    ext; simp [wp, MonadState.set, set, StateT.set, wp_pure, pure, PredTrans.pure,
       PredTrans.pushArg_apply]
 
 theorem EStateM.set_apply (x : σ) :
     wp⟦MonadStateOf.set x : EStateM ε σ PUnit⟧ Q = fun _ => Q.1 ⟨⟩ x := by
-  ext; simp only [wp, MonadState.set, set, EStateM.set, pure_pure, pure, PredTrans.pure,
+  ext; simp only [wp, MonadState.set, set, EStateM.set, wp_pure, pure, PredTrans.pure,
     PredTrans.pushArg_apply]
 
 theorem MonadStateOf.set_apply [MonadStateOf σ m] [MonadLift m n] [WP n _] :
@@ -112,12 +98,12 @@ theorem MonadState.set_apply [WP m sh] [MonadStateOf σ m] :
 
 theorem StateT.modifyGet_apply [Monad m] [WPMonad m ps] (f : σ → α × σ) :
   wp⟦MonadStateOf.modifyGet f : StateT σ m α⟧ Q = fun s => Q.1 (f s).1 (f s).2 := by
-    simp only [wp, MonadStateOf.modifyGet, StateT.modifyGet, pure_pure, pure, PredTrans.pure,
+    simp [wp, MonadStateOf.modifyGet, StateT.modifyGet, wp_pure, pure, PredTrans.pure,
       PredTrans.pushArg_apply]
 
 theorem EStateM.modifyGet_apply (f : σ → α × σ) :
   wp⟦MonadStateOf.modifyGet f : EStateM ε σ α⟧ Q = fun s => Q.1 (f s).1 (f s).2 := by
-      simp only [wp, MonadStateOf.modifyGet, EStateM.modifyGet, pure_pure, pure, PredTrans.pure,
+      simp only [wp, MonadStateOf.modifyGet, EStateM.modifyGet, wp_pure, pure, PredTrans.pure,
       PredTrans.pushArg_apply]
 
 theorem MonadStateOf.modifyGet_apply [MonadStateOf σ m] [MonadLift m n] [WP n _]
